Pollux.Proto.Descriptors.fst
@@ -29,6 +29,16 @@ type pdec =
 | P_OPTIONAL : pdec
 | P_REPEATED : pdec
 
+let sort_pair_fst v1 v2 = (bool_of_compare String.compare) (fst v1) (fst v2)
+let sort_pair_snd v1 v2 = (bool_of_compare String.compare) (snd v1) (snd v2)
+let get_pair_fst l = map fst l
+let get_pair_snd l = map snd l
+let sort_triple_fst (#a:Type) (#b:Type) (v1:string & a & b) (v2:string & a & b) = (bool_of_compare String.compare) (v1._1) (v2._1)
+let get_triple_fst (#a:Type) (#b:Type) (#c:Type) (l:list (a & b & c)) = map (fun (e:a & b & c) -> e._1) l
+let get_triple_snd (#a:Type) (#b:Type) (#c:Type) (l:list (a & b & c)) = map (fun (e:a & b & c) -> e._2) l
+let get_triple_thd (#a:Type) (#b:Type) (#c:Type) (l:list (a & b & c)) = map (fun (e:a & b & c) -> e._3) l
+
+unopteq
 type pty = 
 | P_DOUBLE :           pdec -> pty
 | P_FLOAT :            pdec -> pty 
@@ -40,22 +50,20 @@ type pty =
 | P_BOOL :             pdec -> pty
 | P_STRING :           pdec -> pty
 | P_BYTES :            pdec -> pty
-| P_MSG :              pdec -> pty
+| P_MSG :       m:md -> pdec -> pty
 | P_ENUM :             pdec -> pty
 
-type fd : Type = string & nat & pty
-
-let get_fids (l:list fd) : list nat = map (fun (e : fd) -> e._2) l
-let get_names (l:list fd) : list string = map (fun (e : fd) -> e._1) l
-
-let sort_fd (f1:fd) (f2:fd) : bool = (bool_of_compare String.compare) (f1._1) (f2._1) 
-
-type fields = l:list fd{List.noRepeats (get_fids l) /\ List.noRepeats (get_names l) /\ List.sorted sort_fd l}
-unopteq
-type md : Type = {
+and md : Type = {
   reserved: Set.set nat;
-  fields: fields
+  fields: l:list (string & nat & pty){List.noRepeats (get_triple_fst l) /\ List.noRepeats (get_triple_snd l) /\ List.sorted sort_triple_fst l}
 }
+
+(* 
+  F* doesn't like these as part of the recursive type block, something about needing the unopteq 
+  tag and these not looking recursive enough? Either way, I want these at least as type aliases
+*)
+type fd = string & nat & pty 
+type fields = l:list (string & nat & pty){List.noRepeats (get_triple_fst l) /\ List.noRepeats (get_triple_snd l) /\ List.sorted sort_triple_fst l}
 
 type dvty (v:Type) =
 | VIMPLICIT : v -> dvty v
@@ -69,15 +77,12 @@ type vty =
 | VBOOL     : dvty bool -> vty 
 | VSTRING   : dvty string -> vty 
 | VBYTES    : dvty bytes -> vty 
-| VMSG      : dvty unit -> vty
+| VMSG      : dvty msg -> vty
 | VENUM     : dvty unit -> vty
 
-type vf = string & vty
+and vf = string & vty
 
-let sort_vf (v1:vf) (v2:vf) : bool = (bool_of_compare String.compare) v1._1 v2._1
-
-let msg_names (m:list vf) : list string = map (fun (f:vf) -> f._1) m
-type msg = m:list vf{List.sorted sort_vf m /\ List.noRepeats (msg_names m)} 
+and msg = m:list vf{List.sorted sort_pair_fst m /\ List.noRepeats (get_pair_fst m)} 
 
 let empty_msg : msg = []
 
@@ -87,7 +92,8 @@ let init_dec (#a:Type) (dec:pdec) (def:a) =
   | P_OPTIONAL -> VOPTIONAL None 
   | P_REPEATED -> VREPEATED []
   
-let init_field (f:fd) : vf = f._1, 
+// Refinement needed for proof purposes
+let rec init_field (f:fd) : v:vf{f._1 = v._1} = f._1, 
 (match f._3 with 
  | P_DOUBLE pd -> VDOUBLE (init_dec pd double_z)
  | P_FLOAT pd -> VFLOAT (init_dec pd float_z)
@@ -99,19 +105,18 @@ let init_field (f:fd) : vf = f._1,
  | P_BOOL pd -> VBOOL (init_dec pd false)
  | P_STRING pd -> VSTRING (init_dec pd "")
  | P_BYTES pd -> VBYTES (init_dec pd [])
- | P_MSG pd -> VMSG (init_dec pd ())
- | P_ENUM pd -> VENUM (init_dec pd ())
-)
+ | P_MSG md pd -> VMSG (init_dec pd (init_msg md))
+ | P_ENUM pd -> VENUM (init_dec pd ()))
 
-// Refinement needed for prove purposes
-let rec init_fields (fs:fields) : m:msg{get_names fs = msg_names m} = 
+// Refinement needed for proof purposes
+and init_fields (fs:fields) : m:msg{get_triple_fst fs = get_pair_fst m} = 
   match fs with 
   | [] -> []
   | hd :: tl -> let new_field = init_field hd in  
               let rest_fields = init_fields tl in
               let fields = new_field :: rest_fields in 
-              List.noRepeats_cons new_field._1 (msg_names rest_fields);
-              assert List.noRepeats (msg_names fields);
+              List.noRepeats_cons new_field._1 (get_pair_fst rest_fields);
+              assert List.noRepeats (get_pair_fst fields);
               fields
 
-let init_msg (m:md) : msg = init_fields m.fields 
+and init_msg (m:md) : msg = init_fields m.fields 
